Coq/src/SimRelCert.v
@@ -152,6 +152,8 @@ Section SimRelCert.
 
       tr_step : isim_trav_step G sc ktid TC TC';
 
+      certD_in_cert_ex : cert_dom G TC ktid st ⊆₁ e2a □₁ certX ;
+
       (* TODO : we need to simplify this property somehow *)
       (* hgfix : fixset (ES.cont_sb_dom S k) (h ∘ e2a); *)
 
